
Before demonstrating the claimed facts, let's first establish some technical results.
In this section we will follow the path of proving Lemma 3.1 from \cite{Stich}.

\begin{lemma} \label{lem:lem_1}
    \begin{align*}
        \norm{\bar{x}_t - x_* - \gamma_{t} \bar{g}_t}^2
        &= \norm{\bar{x}_t - x_*}^2 
        + \gamma_{t}^2 \norm{\bar{q}_t 
        + \bar{r}_t - q_* - r_*}^2 
        - 2 \gamma_{t} \inner{\bar{x}_t - x_*}{\bar{q}_t}
        - 2 \gamma_{t} \inner{\bar{x}_t - x_*}{\bar{r}_t} 
    \end{align*}
\begin{proof}
    \begin{align*}
        \norm{\bar{x}_t - x_* - \gamma_{t} \bar{g}_t}^2
        &= 
        \norm{\bar{x}_t - x_*}^2 
        + \gamma_{t}^2 \norm{\bar{g}_t}^2 
        - 2 \gamma_{t} \inner{\bar{x}_t - x_*}{\bar{g}_t} \\
        &= 
        \norm{\bar{x}_t - x_*}^2 
        + \gamma_{t}^2 \norm{\bar{g}_t}^2 
        - \frac{2\gamma_{t}}{M} \summ {m=1}{M}{ \inner{\bar{x}_t - x_*}{\nabla F(x^m_t)} } \\
        &= 
        \norm{\bar{x}_t - x_*}^2 
        + \gamma_{t}^2 \norm{\fsumm {m=1}{M}{\nabla F(x^m_t)}}^2 
        - \frac{2\gamma_{t}}{M} \summ {m=1}{M}{ \inner{\bar{x}_t - x_*}{\nabla F(x^m_t)} } \\
        &= 
            \notag
        \norm{\bar{x}_t - x_*}^2 
        + \gamma_{t}^2 \norm{\fsumm {m=1}{M}{\nabla F(x^m_t)} - \nabla F(x_*)}^2 
        - \frac{2\gamma_{t}}{M} \summ {m=1}{M}{ \inner{\bar{x}_t - x_*}{\nabla F(x^m_t)} } \\
        &= 
            \notag
        \norm{\bar{x}_t - x_*}^2 
        + \gamma_{t}^2 \norm{\fsumm {m=1}{M}{\nabla Q(x^m_t) + \nabla R(x^m_t) - \nabla Q(x_*) - \nabla R(x_*)}}^2  \\
        &- \frac{2\gamma_{t}}{M} \summ {m=1}{M}{ \inner{\bar{x}_t - x_*}{\nabla Q(x^m_t)} }
        - \frac{2\gamma_{t}}{M} \summ {m=1}{M}{ \inner{\bar{x}_t - x_*}{\nabla R(x^m_t)} }  \\
        &= 
        \norm{\bar{x}_t - x_*}^2 
        + \gamma_{t}^2 \norm{\bar{q}_t 
        + \bar{r}_t - q_* - r_*}^2  
        - \frac{2\gamma_{t}}{M} \summ {m=1}{M}{ \inner{\bar{x}_t - x_*}{q^m_t} }
        - \frac{2\gamma_{t}}{M} \summ {m=1}{M} { \inner{\bar{x}_t - x_*}{r^m_t} } \\
        &= 
        \norm{\bar{x}_t - x_*}^2 
        + \gamma_{t}^2 \norm{\bar{q}_t 
        + \bar{r}_t - q_* - r_*}^2 
        - 2 \gamma_{t} \inner{\bar{x}_t - x_*}{\bar{q}_t}
        - 2 \gamma_{t} \inner{\bar{x}_t - x_*}{\bar{r}_t} 
    \end{align*}
\end{proof}
\end{lemma}

\begin{lemma} \label{lem:g_t}
    Bounding the gradient norm
    \[  \norm{\bar{q}_t + \bar{r}_t - q_* - r_*}^2 \\
        \leq
        2 L_Q(1 + \zeta)  (Q(\bar{x}_t) - Q_* - \inner {q_*}{\bar{x}_t - x_*})
        + 2 L_R(1 + \frac{1}{\zeta})  (\bar{R}_t - R_* - \inner {r_*}{\bar{x}_t - x_*})
    \]
\end{lemma}
\begin{proof}
$ $\par
    By the generalized Cauchy inequality:
    \begin{align}
        &\norm{\bar{q}_t + \bar{r}_t - q_* - r_*}^2
        = \norm{\bar{q}_t - q_*}^2 
        + \norm{\bar{r}_t - r_*}^2
        + 2\inner {\bar{q}_t - q_*} {\bar{r}_t - r_*} \label{eq:St_1_1} \\
        &\leq \norm{\bar{q}_t - q_*}^2 
        + \norm{\bar{r}_t - r_*}^2 
        + \zeta \norm{\bar{q}_t - q_*}^2 
        + \frac{1}{\zeta} \norm{\bar{r}_t - r_*}^2 \label{eq:St_1_2} \\
        &= (1 + \zeta)\norm{\bar{q}_t - q_*}^2 + (1 + \frac{1}{\zeta})\norm{\bar{r}_t - r_*}^2  \label{eq:St_1_1}
    \end{align}
    
    By the $L$ - smoothness (corollary~\ref{cor:nesterov}):
    \begin{align}
        (1 + \zeta)\norm{\bar{q}_t - q_*}^2 &+ (1 + \frac{1}{\zeta})\norm{\bar{r}_t - r_*}^2 \\
        &\leq 2 L_Q(1 + \zeta)  (Q(\bar{x}_t) - Q_* - \inner {q_*}{\bar{x}_t - x_*})
        + 2(1 + \frac{1}{\zeta}) L_R (\bar{R}_t - R_* - \inner {r_*}{\bar{x}_t - x_*}) \label{eq:St_1_2}
    \end{align}
    
    Combining together \eqref{eq:St_1_1} and \eqref{eq:St_1_2}, we obtain:
    \begin{align}
        \norm{\bar{q}_t + \bar{r}_t - q_* - r_*}^2 
        \leq 2 L_Q(1 + \zeta)  (Q(\bar{x}_t) - Q_* - \inner {q_*}{\bar{x}_t - x_*})
        + 2 L_R(1 + \frac{1}{\zeta})  (\bar{R}_t - R_* - \inner {r_*}{\bar{x}_t - x_*}) \label{eq:St_1}
    \end{align}
\end{proof}


\begin{lemma} \label{lem:inner_1}
    \begin{align}
        -2 \inner{\bar{x}_t - x_*}{\bar{q}_t} &\leq 2 Q_* - 2 Q(\bar{x}_t) - \mu_Q \norm{\bar{x}_t - x_*}^2 \label{eq:St_2}
    \end{align}
\end{lemma}
\begin{proof}
    By $\mu_Q$ - convexity:
    \begin{align}
        -2 \inner{\bar{x}_t - x_*}{\bar{q}_t} &= 2 \inner{x_* - \bar{x}_t} {\bar{q}_t} \\
        &\leq 2 Q_* - 2 Q(\bar{x}_t) - \mu_Q \norm{\bar{x}_t - x_*}^2
    \end{align}
\end{proof}

\begin{lemma} \label{lem:inner_2}
\begin{align}
    \begin{split}
    - 2 \inner{\bar{x}_t - x_*}{\bar{r}_t} 
    &\leq 
    (\bar{R}_t - R_*)(\frac{1}{p} - 2) + 2 p L_R V_t - \mu_R \norm{x_* - \bar{x}_t}^2 
     - \frac{1}{p}\inner{r_*}{\bar{x}_t - x_*}
    \end{split}
\end{align}
\end{lemma}
\begin{proof}
    \begin{align}
        - 2 \inner{\bar{x}_t - x_*}{\bar{r}_t} &= 2 \inner{x_* - \bar{x}_t} {\bar{r}_t} \\
        &= \frac{2}{M} \summ{m=1}{M}{ \inner{x_* - \bar{x}_t}{r^m_t} } 
        = \frac{2}{M} \summ{m=1}{M}{\inner{x_* - x^m_t + x^m_t - \bar{x}_t}{r^m_t}} \\
        &= \frac{2}{M} \summ{m=1}{M}{\inner{x_* - x^m_t}{r^m_t}} 
        + \frac{2}{M} \summ{m=1}{M}{\inner{x^m_t - \bar{x}_t}{r^m_t}} \label{eq:St_3_0}
    \end{align}
    
    First part, by $\mu_R$ - convexity and Jensen's inequality:
    \begin{align}
        &\frac{2}{M} \summ{m=1}{M}{\inner{x_* - x^m_t}{r^m_t}} 
        \leq \frac{1}{M} \summ{m=1}{M}{2 R_* - 2 R(x^m_t) - \mu_R \norm{x_* - x^m_t}^2} \\
        &\leq \frac{1}{M} \summ{m=1}{M}{2 R_* - 2 R(x^m_t) - \mu_R \norm{x_* - \bar{x}_t}^2} 
        = 2 R_* - 2 \bar{R}_t - \mu_R \norm{x_* - \bar{x}_t}^2 \label{eq:St_3_1}
    \end{align}
    
    Second part, by the generalized Cauchy inequality:
    \begin{align}
        &\frac{2}{M} \summ{m=1}{M}{\inner{x^m_t - \bar{x}_t}{r^m_t}}
        = \frac{2}{M} \summ{m=1}{M}{\inner{x^m_t - \bar{x}_t}{r^m_t - r_*}} 
        + \frac{2}{M} \summ{m=1}{M}{\inner{x^m_t - \bar{x}_t}{r_*}} \\
        &= 
        \frac{2}{M} \summ{m=1}{M}{\inner{x^m_t - \bar{x}_t}{r^m_t - r_*}} 
        \leq \frac{2}{M} \summ{m=1}{M}{p L_R \norm{x^m_t - \bar{x}_t}^2 }
        + \frac{1}{M} \summ{m=1}{M}{\frac{1}{2 p L_R} \norm{r^m_t-r_*}^2 } \\
        &= 
        2 p L_R V_t 
        + \frac{1}{M} \summ{m=1}{M}{\frac{1}{2 p L_R} \norm{r^m_t-r_*}^2 } \label{eq:St_3_2_1}
    \end{align}
    
    By the corollary~\ref{cor:nesterov}:
    \begin{align}
        \norm{r^m_t-r_*}^2 \leq 2L_R (R(x^m_t) - R_* - \inner {r_*}{x^m_t - x_*}) \label{eq:St_3_2_2}
    \end{align}
    
    Substituting \eqref{eq:St_3_2_2} into \eqref{eq:St_3_2_1}, we complete the second part:
    \begin{align}
        &\frac{2}{M} \summ{m=1}{M}{\inner{x^m_t - \bar{x}_t}{r^m_t}}
        \leq 2 p L_R V_t 
        + \frac{1}{pM} \summ{m=1}{M}{R(x^m_t) - R_* - \inner {r_*}{x^m_t - x_*} } \\
        &\leq 2 p L_R V_t 
        + \frac{1}{p} (\bar{R}_t - R_* - \inner {r_*}{\bar{x}_t - x_*}) \label{eq:St_3_2}
    \end{align}
    
    Combining together \eqref{eq:St_3_0}, \eqref{eq:St_3_1}, \eqref{eq:St_3_2}, we gain:
    \begin{align}
         - 2 \inner{\bar{x}_t - x_*}{\bar{r}_t} &\leq
         2 R_* - 2 \bar{R}_t - \mu_R \norm{x_* - \bar{x}_t}^2 
         + 2 p L_R V_t + \frac{1}{p} (\bar{R}_t - R_* - \inner {r_*}{\bar{x}_t - x_*}) \\ 
         &= (\bar{R}_t - R_*)(\frac{1}{p} - 2) + 2 p L_R V_t - \mu_R \norm{x_* - \bar{x}_t}^2 
         - \frac{1}{p}\inner{r_*}{\bar{x}_t - x_*}
         \label{eq:St_3}
    \end{align}
\end{proof}

\begin{lemma}\label{lem:AB-lemma}
    \begin{align}
    \begin{split}
        &\norm{\bar{x}_t - x_* - \gamma_{t} \bar{g}_t}^2 \leq \\
        &(1 - \gamma_{t} \mu)\norm{\bar{x}_t - x_*}^2 + 2 \gamma_{t} p L_R V_t \\
        &+ 2\gamma_{t} (A(\zeta) - 1)(Q(\bar{x}_t) - Q_*) \\
        &+ 2\gamma_{t} (B(\zeta) - 1)(\bar{R}_t - R_*) \\
        &- 2\gamma_{t} A(\zeta) \inner{q_*}{\bar{x}_t - x_*} \\
        &- 2\gamma_{t} B(\zeta) \inner{r_*}{\bar{x}_t - x_*}
    \end{split}
\end{align}
Where $A$ and $B$ are functions of $\zeta \in \mathbb{R}$ such that:
\[A(\zeta) = \gamma_{t} L_Q(1+\zeta)\] 
\[B(\zeta) = \gamma_{t} L_R(1+\frac{1}{\zeta}) + \frac{1}{2p}\]

\end{lemma}
\begin{proof} Substituting the results of Lemmas~\ref{lem:g_t},~\ref{lem:inner_1} and~\ref{lem:inner_2} into Lemma~\ref{lem:lem_1} and doing some algebraic manipulations:
    \begin{align}
        \begin{split}
            &\norm{\bar{x}_t - x_* - \gamma_{t} \bar{g}_t}^2 \leq \norm{\bar{x}_t - x_*}^2 \\
            &+ 2\gamma_{t}^2 L_Q (1 + \zeta) (Q(\bar{x}_t) - Q_* - \inner {q_*}{\bar{x}_t - x_*}) \\
            &+ 2\gamma_{t}^2 L_R (1 + \frac{1}{\zeta}) (\bar{R}_t - R_* - \inner {r_*}{\bar{x}_t - x_*}) \\
            &+ \gamma_{t} ( 2 Q_* - 2 Q(\bar{x}_t) - \mu_Q \norm{\bar{x}_t - x_*}^2 ) \\
            &+ \gamma_{t}(\bar{R}_t - R_*)(\frac{1}{p} - 2) + 2 \gamma_{t} p L_R V_t - \gamma_{t} \mu_R \norm{x_* - \bar{x}_t}^2 - \frac{\gamma_{t}}{p}\inner{r_*}{\bar{x}_t - x_*}\\
            &= (1 - \gamma_{t} \mu_Q - \gamma_{t} \mu_R)\norm{\bar{x}_t - x_*}^2 + 2 \gamma_{t} p L_R V_t \\
            &+ (Q(\bar{x}_t) - Q_*)\coef {2\gamma_{t}^2 L_Q (1+\zeta) - 2\gamma_{t}}
            + (\bar{R}_t - R_*)\coef{2\gamma_{t}^2 L_R (1+\frac{1}{\zeta}) - 2\gamma_{t} + \frac{\gamma_{t}}{p}} \\
            &- 2\inner{q_*}{\bar{x}_t - x_*}\coef{\gamma_{t}^2 L_Q(1+\zeta)}
            - 2\inner{r_*}{\bar{x}_t - x_*}\coef{\gamma_{t}^2 L_R(1+\frac{1}{\zeta}) + \frac{\gamma_{t}}{2p}} \label{eq:lol}
        \end{split}
    \end{align}
    
    Utilizing that $\mu_Q + \mu_R = \lambda$ \eqref{eq:lol}
    \begin{align}
        \begin{split}
             &\norm{\bar{x}_t - x_* - \gamma_{t} \bar{g}_t}^2 \leq 
            (1 - \gamma_{t} \lambda)\norm{\bar{x}_t - x_*}^2 + 2 \gamma_{t} p L_R V_t \\
            &+ (Q(\bar{x}_t) - Q_*)\coef {2\gamma_{t}^2 L_Q (1+\zeta) - 2\gamma_{t}}
            + (\bar{R}_t - R_*)\coef{2\gamma_{t}^2 L_R (1+\frac{1}{\zeta}) - 2\gamma_{t} + \frac{\gamma_{t}}{p}} \\
            &- 2\inner{q_*}{\bar{x}_t - x_*}\coef{\gamma_{t}^2 L_Q(1+\zeta)}
            - 2\inner{r_*}{\bar{x}_t - x_*}\coef{\gamma_{t}^2 L_R(1+\frac{1}{\zeta}) + \frac{\gamma_{t}}{2p}} \\
            &= (1 - \gamma_{t} \lambda)\norm{\bar{x}_t - x_*}^2 + 2 \gamma_{t} p L_R V_t \\
            &+ 2\gamma_{t} (Q(\bar{x}_t) - Q_*)\coef{\gamma_{t} L_Q (1+\zeta) - 1} 
            + 2\gamma_{t} (\bar{R}_t - R_*)\coef{\gamma_{t} L_R (1+\frac{1}{\zeta}) - 1 + \frac{1}{2p}} \\
            &- 2\gamma_{t} \inner{q_*}{\bar{x}_t - x_*}\coef{\gamma_{t} L_Q(1+\zeta) }
            - 2\gamma_{t} \inner{r_*}{\bar{x}_t - x_*}\coef{\gamma_{t} L_R(1+\frac{1}{\zeta}) + \frac{1}{2p}}
        \end{split}
    \end{align}
        
By substituting the expressions in square brackets with $A$ and $B$, we obtain the statement of the lemma.
\end{proof}

\begin{lemma}\label{lem:Technical}
    Exists $\zeta_1$ such that $A(\zeta_1) = B(\zeta_1)$ and $A(\zeta_1) - 1 \leq 0$
\end{lemma}
\begin{sublemma}\label{sublem:sublemma_1}
    Exists $\zeta_1$ such that $A(\zeta_1) = B(\zeta_1)$
\end{sublemma}
\begin{proof}
    By equating $A$ and $B$, we obtain the chain of equalities:

    \begin{align}
        &\gamma_{t} L_Q(1+\zeta)= \gamma_{t} L_R(1+\frac{1}{\zeta}) + \frac{1}{2p} \\
        &L_Q(1+\zeta) = L_R(1+\frac{1}{\zeta}) + \frac{1}{2\gamma_{t} p} \\
        &L_Q + \zeta L_Q - L_R - \frac{L_R}{\zeta} - \frac{1}{2\gamma_{t} p} = 0 \\
        &\zeta L_Q + \zeta^2 L_Q - \zeta L_R - L_R - \frac{\zeta}{2\gamma_{t} p} = 0\\
        &\zeta^2 L_Q + \zeta (L_Q - L_R - \frac{1}{2\gamma_{t} p}) - L_R = 0 \\
        &\zeta_{1} := \frac{-(L_Q - L_R - \frac{1}{2\gamma_{t} p}) + \sqrt{(L_Q - L_R - \frac{1}{2\gamma_{t} p})^2 + 4 L_Q L_R}}{2L_Q} > 0
    \end{align}
    
    $\zeta_{1}$ is a solution to a quadratic equation. Thus,
    \begin{align}
        \gamma_{t} L_R (1+\frac{1}{\zeta_1}) + \frac{1}{2p} = \gamma_{t} L_Q (1+\zeta_1) \label{eq:St_5}
    \end{align}
\end{proof}


\begin{sublemma}\label{sublem:sublemma_2}
    For $\zeta_1$ from previous lemma: $A(\zeta_1) - 1 \leq -\frac{1}{12} \leq 0$
\end{sublemma}
\begin{proof}
    Let us take $\gamma_{t} \leq \frac{1}{6 L}$, meaning that $L \leq \frac{1}{6 \gamma_{t} }$:
    \begin{align}
        A(\zeta_1)& - 1 = \gamma_{t} L_Q(1+\zeta_1) - 1 \\
        &= \gamma_{t} L_Q 
        \coef {1 + \frac{-(L_Q - L_R - \frac{1}{2\gamma_{t} p})+\sqrt{(L_Q - L_R -\frac{1}{2\gamma_{t} p})^2 + 4 L_Q L_R}}{2L_Q} } - 1\\
        &=
        \frac{\gamma_{t}}{2} 
        \coef {2L_Q - (L_Q - L_R - \frac{1}{2\gamma_{t} p}) + \sqrt{(L_Q - L_R - \frac{1}{2\gamma_{t} p})^2 + 4 L_Q L_R} } - 1\\ 
        & \leq
        \frac{\gamma_{t}}{2} 
        \coef {|L_Q + L_R + \frac{1}{2\gamma_{t} p}| + |L_Q - L_R - \frac{1}{2\gamma_{t} p}| + \sqrt{ 4 L_Q L_R} } - 1\\
        & \leq
        \frac{\gamma_{t}}{2} 
        \coef {L_Q + L_R + \frac{1}{2\gamma_{t} p} + L + \frac{1}{2\gamma_{t} p} + \sqrt{ 4 L^2} } - 1\\
        & \leq
        \frac{\gamma_{t}}{2} 
        \coef {5 L + \frac{1}{\gamma_{t} p} } - 1
        \leq
        \frac{\gamma_{t}}{2} 
        \coef {\frac{5}{6 \gamma_{t}} + \frac{1}{\gamma_{t} p} } - 1 \\
        &=
        \frac{5}{12} + \frac{1}{2p} - 1
        = \frac{1}{2p} - \frac{7}{12}
    \end{align}
    
    For $p \geq 1$:
    \begin{align}
         \gamma_{t} L_Q(&1+\zeta_1) - 1 \leq \frac{1}{2p} - \frac{7}{12} \leq \frac{6}{12} - \frac{7}{12} 
         = -\frac{1}{12} < 0 \label{eq:St_6}
    \end{align}
\end{proof}

Combining the results of Sublemmas~\ref{sublem:sublemma_1} and~\ref{sublem:sublemma_2}, 
we obtain the statement of Lemma ~\ref{lem:Technical}.

Further, let's denote $A(\zeta_1)$ as $A_1$ and $B(\zeta_1)$ as $B_1$
\begin{lemma} \label{lem:main}
    Generalization of Lemma 3.1 from \cite{Stich}.
    \begin{align}
        \begin{split}
            \norm{\bar{x}_t - x_* - \gamma_{t} \bar{g}_t}^2 
            \leq (1 - \gamma_{t} \mu)\norm{\bar{x}_t - x_*}^2  - \frac{\gamma_{t}}{6} (F(\bar{x}_t) - F_*) + 2 \gamma_{t} L_R V_t
        \end{split}
    \end{align}
\end{lemma}
\begin{proof}
    From Lemma~\ref{lem:AB-lemma} we know that:
    \begin{align}
        \begin{split}
            \norm{\bar{x}_t - x_* - \gamma_{t} \bar{g}_t}^2 \leq \\
            &(1 - \gamma_{t} \lambda)\norm{\bar{x}_t - x_*}^2 + 2 \gamma_{t} p L_R V_t \\
            &+ 2\gamma_{t} (A - 1)(Q(\bar{x}_t) - Q_*)
            + 2\gamma_{t} (B - 1)(\bar{R}_t - R_*) \\
            &- 2\gamma_{t} A \inner{q_*}{\bar{x}_t - x_*}
            - 2\gamma_{t} B \inner{r_*}{\bar{x}_t - x_*} \label{eq:main}
        \end{split}
    \end{align}
    Using the result of Lemma~\ref{lem:Technical}, and substituting $\zeta_1$ into $A$ and $B$, we obtain that 
    $A(\zeta_1) = B(\zeta_1) \ = A_1 = B_1$:
    \begin{align}
        - 2\gamma_{t} A_1 \inner{q_*}{\bar{x}_t - x_*} - 2\gamma_{t} B_1 \inner{r_*}{\bar{x}_t - x_*} 
        &= - 2\gamma_{t} A_1 \inner{q_* + r_*}{\bar{x}_t - x_*} \\
        &= - 2\gamma_{t} A_1 \inner{\nabla F(x_*)}{\bar{x}_t - x_*} = 0 \label{eq:zero}
    \end{align}

    For $a \geq 0$ by Jensen's inequality:
    \begin{align}
        -a (\fsumm{m=1}{M}{R(x^m_t}) - R_*) \leq -a (R(\bar{x}_t) - R_*) \label{eq:jensen'} 
    \end{align}
    
    Using that $A_1 - 1 \leq 0$ allows us to use \eqref{eq:jensen'}:
    \begin{align}
        2\gamma_{t} (B_1 - 1)(\bar{R}_t - R_*) &= 2\gamma_{t} (A_1 - 1)(\bar{R}_t - R_*) \\
        &= |2\gamma_{t} (A_1 - 1)| \cdot (R_* - \bar{R}_t) = |2\gamma_{t} (A_1 - 1)| \cdot (R_* - \fsumm{m=1}{M}{R(x^m_t})) \\
        &\leq |2\gamma_{t} (A_1 - 1)| \cdot (R_* - R(\bar{x}_t)) = 2\gamma_{t} (A_1 - 1) (R(\bar{x}_t) - R_*) \label{eq:jensen}
    \end{align}
    
    Substituting \eqref{eq:zero} and \eqref{eq:jensen} into \eqref{eq:main}:
    \begin{align}
        &\norm{\bar{x}_t - x_* - \gamma_{t} \bar{g}_t}^2 \\
        &\leq (1 - \gamma_{t} \lambda)\norm{\bar{x}_t - x_*}^2 + 2 \gamma_{t} p L_R V_t
        + 2\gamma_{t} (A_1 - 1)(Q(\bar{x}_t) - Q_* + R(\bar{x}_t) - R_*) \\
        &= (1 - \gamma_{t} \lambda)\norm{\bar{x}_t - x_*}^2 + 2 \gamma_{t} p L_R V_t
        + 2\gamma_{t} (A_1 - 1)(F(\bar{x}_t) - F_*)
    \end{align}
    
    Given that Lemma~\ref{lem:Technical} holds for $p = 1$, we can combine the result of Sublemma~\ref{sublem:sublemma_2} with the fact that $F(\bar{x}_t) - F_* \geq 0$ to further strengthen our argument:
    
    \begin{align}
        \norm{\bar{x}_t - x_* - \gamma_{t} \bar{g}_t}^2 &
        \leq (1 - \gamma_{t} \lambda)\norm{\bar{x}_t - x_*}^2 + 2 \gamma_{t} L_R V_t
        + 2\gamma_{t} (A_1 - 1)(F(\bar{x}_t) - F_*) \\
        &\leq (1 - \gamma_{t} \lambda)\norm{\bar{x}_t - x_*}^2 - 2\gamma_{t} \frac{1}{12}(F(\bar{x}_t) - F_*) + 2 \gamma_{t} L_R V_t
    \end{align}
    Thus completing the proof.
\end{proof}


Now we will present the final result of the Subsection:


\begin{lemma} \label{lem:very_main}
    For $\gamma_{t} \leq \frac{1}{6L}$:
    \begin{align}
        \E \norm{\bar{x}_{t+1}-x_*}^2
        &\leq (1 - \gamma_{t} \lambda) \E \norm{\bar{x}_t - x_*}^2 
        + \gamma_{t}^2 \E \norm{ \bar{\mc{g_t}} - \bar{g}_t}^2
        - \frac{\gamma_{t}}{6} \E [F(\bar{x}_t) - F_*] 
        + 2 \gamma_{t} L_R \E [V_t]
    \end{align}
\end{lemma}
\begin{proof}
    Using the update equation \eqref{eq:upd_eq} we have
    \begin{align}
        \norm{\bar{x}_{t+1}-x_*}^2
        &= \norm{\bar{x}_{t} - \gamma_{t} \bar {\mc{g_t}} - x_*}^2
        = \norm{\bar{x}_{t} - \gamma_{t} \bar {\mc{g_t}} - x_* - \gamma_{t} \bar{g}_t + \gamma_{t} \bar{g}_t}^2 \\
        &= \norm{\bar{x}_t - x_* - \gamma_{t} \bar{g}_t}^2 
        + \gamma_{t}^2 \norm{\bar {\mc{g_t}} - \bar{g}_t}^2
        - 2 \gamma_{t} \inner{\bar{x}_t - x_* - \gamma_{t} \bar{g}_t}{\bar {\mc{g_t}} - \bar{g}_t}
    \end{align}
    
    Taking expectation, 
    \begin{align}
        \E \norm{\bar{x}_{t+1}-x_*}^2
        &= \E \norm{\bar{x}_t - x_* - \gamma_{t} \bar{g}_t}^2
        + \gamma_{t}^2 \E \norm{ \bar {\mc{g_t}} - \bar{g}_t}^2 \label{eq:2204_3}
    \end{align}
    
    
    Taking expectiation of result of Lemma~\ref{lem:main}:
    \begin{align}
        \E \norm{\bar{x}_t - x_* - \gamma_{t} \bar{g}_t}^2 
        &\leq (1 - \gamma_{t} \lambda) \E \norm{\bar{x}_t - x_*}^2 
        - \frac{\gamma_{t}}{6} \E [F(\bar{x}_t) - F_*] 
        + 2 \gamma_{t} L_R \E [V_t] \label{eq:2204_2}
    \end{align}

    Combination of \eqref{eq:2204_3} and \eqref{eq:2204_2} yields the claim of the Lemma:
    \begin{align}
         \E \norm{\bar{x}_{t+1}-x_*}^2
        &\leq (1 - \gamma_{t} \lambda) \E \norm{\bar{x}_t - x_*}^2 
        + \gamma_{t}^2 \E \norm{ \bar{\mc{g_t}} - \bar{g}_t}^2
        - \frac{\gamma_{t}}{6} \E [F(\bar{x}_t) - F_*] 
        + 2 \gamma_{t} L_R \E [V_t]
    \end{align}
\end{proof}